no progress just moving stuff around

src/arch/x64/X64.Vale.StrongPost_i.fst
@@ -141,4 +141,4 @@ let va_lemma_strong_post_norm inss s0 sN =
   assert_to_norm (strong_post inss s0 sN);
   ()
 
-let va_lemma_wp_norm inss post s0 = admit ()
+let lemma_weakest_pre_norm inss s0 = admit ()
