src/arch/x64/X64.Vale.StrongPost_i.fsti
@@ -149,56 +149,6 @@ let rec strong_post (inss:list ins) (s0:state) (sN:state) : Type0 =
         strong_post inss ({update_reg dst x s0 with flags = f}) sN)  
   | _ -> True
 
-[@"opaque_to_smt"]
-let rec wp_code (inss : list ins) (post: state -> Type0) (s0:state): Type0 = 
-    match inss with
-    | [] -> 
-      (forall okN regsN flagsN memN. 
-        let sN = {ok=okN; regs=regsN; flags=flagsN; mem=memN} in
-          ( (~(okN == s0.ok /\
-             memN == s0.mem /\
-            flagsN == s0.flags /\
-            all_regs_match s0 sN)) \/
-            post sN))
-    (* | (Mov64 (OReg Rsp) _) :: _ -> False *)
-    (* | (Mov64 (OReg dst) src) :: inss -> *)
-    (*   valid_operand_norm src s0 /\ *)
-    (*   (forall x. x == eval_operand_norm src s0 ==> *)
-    (*         wp_code inss post (update_reg dst x s0)) *)
-    (*   (\* let post' = wp_code inss post in *\) *)
-    (*   (\* (valid_operand_norm src s0) /\ *\) *)
-    (*   (\* post' (update_reg dst (eval_operand_norm src s0) s0) *\) *)
-    (* | (Load64 (OReg Rsp) _ _) :: inss -> False *)
-    | (Load64 (OReg dst) (OReg src) offset) :: inss ->
-      mem_contains s0.mem (s0.regs src + offset) /\
-      (forall x.
-        ~ (x == mem_sel s0.mem (s0.regs src + offset)) \/
-        wp_code inss post (update_reg dst x s0))
-    (* | (Store64 (OReg dst) src offset) :: inss -> *)
-    (*   let post' = wp_code inss post in *)
-    (*   (valid_operand_norm src s0) /\ *)
-    (*   (mem_contains s0.mem (s0.regs dst + offset)) /\ *)
-    (*   post' (update_mem (s0.regs dst + offset) (eval_operand_norm src s0) s0) *)
-    (* | (Add64Wrap (OReg Rsp) _) :: inss -> wp_code inss post s0 *)
-    // | (Add64Wrap (OReg dst) src) :: inss ->
-    //   let post' = wp_code inss post in
-    //   (valid_operand_norm src s0) /\
-    //   (forall a x f. 
-    //     (~ (a == s0.regs dst + eval_operand_norm src s0 /\
-    //           x == (if a < nat64_max then a else a - nat64_max) /\
-    //           cf f == (a >= nat64_max))) \/
-    //     post' ({update_reg dst x s0 with flags = f}))
-    // | (Adc64Wrap (OReg Rsp) _) :: inss -> wp_code inss post s0
-    // | (Adc64Wrap (OReg dst) src) :: inss ->
-    //   let post' = wp_code inss post in
-    //   (valid_operand_norm src s0) /\
-    //   (forall a x f.
-    //   (~ (a == s0.regs dst + eval_operand_norm src s0 + (if cf s0.flags then 1 else 0) /\
-    //       x == (if a < nat64_max then a else a - nat64_max) /\
-    //       cf f == (a >= nat64_max))) \/
-    //     post' ({update_reg dst x s0 with flags = f}))
-    | _ -> True
-
 let rec inss_to_codes (inss:list ins) : list va_code =
   match inss with
   | (Mov64 (OReg Rsp) _)::inss -> []
@@ -221,6 +171,35 @@ let rec inss_to_codes (inss:list ins) : list va_code =
   | (Sub64 (OReg dst) src)::inss -> (va_code_Sub64 (OReg dst) src)::(inss_to_codes inss)
   | _ -> []
 
+[@"opaque_to_smt"]
+let rec wp_code (inss : list ins) (post: state -> Type0) (s0:state): Type0 = 
+  match inss with
+  | [] -> 
+       (forall okN regsN flagsN memN.
+       let sN = {ok=okN; regs=regsN; flags=flagsN; mem=memN} in
+       okN == s0.ok /\
+       memN == s0.mem /\
+       flagsN == s0.flags /\
+       all_regs_match s0 sN ==>
+       post sN)
+  | (Mov64 (OReg Rsp) _) :: _ -> False
+  | (Mov64 (OReg dst) src) :: inss ->
+    valid_operand_norm src s0 /\
+    (forall x. x == eval_operand_norm src s0 ==>
+          wp_code inss post (update_reg dst x s0))
+  | (Load64 (OReg Rsp) _ _) :: inss -> False
+  | (Load64 (OReg dst) (OReg src) offset) :: inss ->
+    mem_contains s0.mem (s0.regs src + offset) /\
+    (forall x. x == mem_sel s0.mem (s0.regs src + offset) ==>
+          wp_code inss post (update_reg dst x s0))
+  | (Store64 (OReg dst) src offset) :: inss ->
+    (valid_operand_norm src s0) /\
+    (mem_contains s0.mem (s0.regs dst + offset)) /\
+    (forall x. x == eval_operand_norm src s0 ==>
+      wp_code inss post (update_mem (s0.regs dst + offset) x s0)) 
+  | _ -> True
+
+
 val va_lemma_strong_post_norm : inss:list ins -> s0:state -> sN:state -> Lemma
   (requires
     Some sN == va_eval_code (va_Block (normalize_term (inss_to_codes inss))) s0 /\
@@ -233,3 +212,26 @@ val va_lemma_strong_post_norm : inss:list ins -> s0:state -> sN:state -> Lemma
       normalize (strong_post inss
         ({ok = ok0; regs = regs0; flags = flags0; mem = mem0})
         ({ok = okN; regs = regsN; flags = flagsN; mem = memN})))
+
+let wp_code_delta = [
+  "X64.Vale.StrongPost_i.wp_code";
+  "X64.Vale.StrongPost_i.all_regs_match";
+  "X64.Vale.StrongPost_i.regs_match";
+  "X64.Vale.StrongPost_i.eval_operand_norm";  
+  "X64.Vale.State_i.update_reg'";
+  "X64.Vale.State_i.__proj__Mkstate__item__regs";
+  "X64.Vale.State_i.__proj__Mkstate__item__ok" ;
+  "X64.Vale.State_i.__proj__Mkstate__item__flags"; 
+  "X64.Vale.State_i.__proj__Mkstate__item__mem"; 
+  ]
+
+val lemma_weakest_pre_norm: inss:list ins -> s0:state -> PURE state
+  (fun (post:(state -> Type)) ->
+     forall ok0 regs0 flags0 mem0. 
+        ok0 == s0.ok /\
+        regs0 == s0.regs /\
+        flags0 == s0.flags /\
+        mem0 == s0.mem ==>
+        s0.ok /\
+        Prims.norm [delta_only wp_code_delta; zeta; iota; primops]
+                   (wp_code inss post ({ok=ok0; regs=regs0; flags=flags0; mem=mem0})))
